\documentclass[10pt,a4paper,draft]{article}
\usepackage[utf8]{inputenc}
\usepackage{amsmath}
\usepackage{amsfonts}
\usepackage{amssymb}
\begin{document}
\begin{flushleft}
\section{Syntax}

\begin{align*}
\text{Expressions }e \; ::= \; &varident  \\
&| \; num \; n \; | \; false \; | \; true \\
&|\;e_{1}e_{2} \\
&|\;(e_{1},e_{2}) \\
&|\;\lambda(p)\;.\;e \\
&|\;let \; p \; = \; e_{1} \; in \; e_{2} \\
&|\;letrec \; p \; = \; e_{1} \; in \; e_{2} \\
&|\; if(e_{1}) \; then \; e_{2} \; else \; e_{3}\\
\\
\text{Pattern }p \; ::= \; &varident \\
&| \; (p,p)
\end{align*}

\section{Type System}

\begin{align*}
\text{Types }\tau \; ::= \; &nat \\
&| \; bool \\
&| \; \tau_{1} \rightarrow \tau_{2} \\
&| \; \tau_{1} \times \tau_{2} \\
&| \; \alpha \\
\\
\text{Type-Schemes } \sigma \; ::= \; &\tau \\
&| \; \forall \alpha . \sigma \\
\\
\text{Context }\Gamma ::=\; &\cdot \\
&| \; \Gamma :(x:\tau) \\
\\
\text{Typing } ::=\;&\Gamma \vdash e: \sigma \\
\end{align*}

\subsection{Rules}
\begin{align*}
&\Gamma \vdash true : bool \tag{T-True} \\
&\Gamma \vdash false : bool \tag{T-False} \\
&\Gamma \vdash num \; n : nat \tag{T-Num} \\ \\
\tag{T-Mono}
&\frac{\sigma \geq \tau \;\;\;\;\;\; \Gamma \vdash varident:\sigma}{\Gamma \vdash varident:\tau}\\ \\
\tag{T-App}
&\frac{\Gamma \vdash e_{1}:\tau_{2} \rightarrow \tau_{1} \;\;\;\;\;\; \Gamma \vdash e_{2}:\tau_{2}}
{\Gamma \vdash e_{1}e_{2}:\tau_{1}} \\ \\
\tag{T-BuildContext1}
& varident:\sigma \rightarrow \cdot:(varident):\sigma \\ \\
\tag{T-BuildContext2}
&\frac{p_{1}:\sigma_{1} \rightarrow \Gamma_{1} \;\;\;\;\;\; p_{2}:\sigma_{2}\rightarrow \Gamma_{2} \;\;\;\;\;\; \Gamma_{3} = \Gamma_{1}\bigcup \Gamma_{2}}{(p_{1},p_{2}):\sigma_{1}\times \sigma_{2} \rightarrow \Gamma_{3}} \\ \\
\tag{T-Fun}
&\frac{p:\tau_{2} \rightarrow \Gamma_{2} \;\;\;\;\;\; \Gamma_{2} \bigcup \Gamma_{1} \vdash e:\tau_{1}}
{\Gamma_{1} \vdash \lambda(p).e:\tau_{2} \rightarrow \tau_{1}} \\ \\
\tag{T-IfThenElse}
&\frac{\Gamma \vdash e_{1}:bool \;\;\;\;\;\; \Gamma \vdash e_{2}:\tau \;\;\;\;\;\; \Gamma \vdash e_{3} : \tau}
{\Gamma \vdash if \; e_{1} \; then \; e_{2} \; else \; e_{3} : \tau} \\ \\
\tag{T-Pair}
&\frac{\Gamma \vdash e_{1}:\tau_{1} \;\;\;\;\;\; \Gamma \vdash e_{2}:\tau_{2}}
{\Gamma \vdash (e_{1},e_{2}) : \tau_{1}\times\tau_{2}} \\ \\
\tag{T-Let}
&\frac{\Gamma \vdash e_{2}:\tau_{2} \;\;\; \sigma=gen(\Gamma,\tau)\;\;\;p:\sigma\rightarrow \Gamma_{2} \;\;\; \Gamma \bigcup \Gamma_{2} \vdash e_{1}:\tau}
{\Gamma \vdash let\;p\;=\;e_{2}\;in\;e_{1}:\tau} \\ \\
\tag{T-Letrec}
&\frac{\Gamma \vdash let\;p\;=\;fix\;(\lambda p.e_{2})\;in\;e_{1}:\tau}
{\Gamma \vdash letrec\;p\;=\;e_{2}\;in\;e_{1}:\tau} \\ \\
\tag{T-Fix}
&\frac{\Gamma \vdash e : \tau \rightarrow \tau}
{\Gamma \vdash fix(e) : \tau}
\end{align*}

\section{Operational semantics}
\begin{align*}
\text{Values }v ::=\;&num n \; | \; true \; | \; false \\
&| (v,v) \\
&| \lambda p.e\\
\\
\text{Evaluation } ::= &e \rightarrow e' \\
\end{align*}
\subsection{Rules}
\begin{align*}
\tag{E-IfTrue}
&if \; true  \; then \; e_{1} \; else \; e_{2} \rightarrow e_{1}\\
\tag{E-IfFalse}
&if \; false \; then \; e_{1} \; else \; e_{2} \rightarrow e_{2}\\ \\
\tag{E-IfThenElse}
&\frac{e_{1} \rightarrow e_{1}'}
{if \; e_{1} \; then \; e_{2} \; else \; e_{3} \rightarrow if \; e_{1}' \; then \; e_{2} \; else \; e_{3}}\\ \\
\tag{E-PairLeft}
&\frac{e_{1} \rightarrow e_{1}'}
{(e_{1},e_{2}) \rightarrow (e_{1}',e_{2})} \\ \\
\tag{E-PairRight}
&\frac{e_{2} \rightarrow e_{2}'}
{(e_{1},e_{2}) \rightarrow (e_{1},e_{2}')} \\ \\
\tag{E-Let}
&\frac{e_{1}\rightarrow e_{1}'}
{let \; p \; = \; e_{1} \; in \; e_{2} \rightarrow let \; x \; = \; e_{1}' \; in \; e_{2}}
\\ \\
\tag{E-LetV}
&let \; x \; = \; v \; in \; e \rightarrow [x \mapsto v]e \\ \\
\tag{E-LetRec}
&letrec\;p=\;e_{1} \; in \; e_{2} \rightarrow let \; p \; = fix(\lambda p.e_{1}) \; in \; e_{2} \\ \\ 
\tag{E-Fix}
&\frac{e\rightarrow e'}
{fix(e) \rightarrow fix(e')}\\ \\
\tag{E-FixRec}
&fix(\lambda(p.e)) \rightarrow [p \mapsto (fix (\lambda(p.e))]e \\ \\
\tag{E-PatternMatch}
&let \; (p_{1},p_{2}) \; = \; (e_{1},e_{2}) \; in \; e_{3} \rightarrow
let \; p_{1} \; = \; e_{1} \; in \;
(let \; p_{2}  \; = \; e_{2} \; in \; e_{3}) \\ \\
\tag{E-App1}
&\frac{e_{1} \rightarrow e_{1}'}
{e_{1} e_{2} \rightarrow e_{1}' e_{2}}\\ \\
\tag{E-App2}
&\frac{e_{2} \rightarrow e_{2}'}
{v\;e_{2} \rightarrow v\;e_{2}'}\\ \\
\tag{E-Lambda}
&(\lambda x . e) \; v \rightarrow [x \mapsto v]e \\ \\
\tag{E-MatchLambda}
&(\lambda (p_{1},p_{2}) . e_{3}) \; (e_{1},e_{2}) \rightarrow (\lambda p_{1}.(\lambda p_{2}.e_{3})\;e_{2})\; e_{1}
\end{align*}
\end{flushleft}
\end{document}