\begin{figure}[htb]
\begin{align*}
%\tag{E-IfTrue}
%&T \vdash if \; true  \; then \; e_{1} \; else \; e_{2} \rightarrow T \vdash e_{1}\\
%\tag{E-IfFalse}
%&T \vdash if \; false \; then \; e_{1} \; else \; e_{2} \rightarrow T \vdash e_{2}\\ \\
%\tag{E-IfThenElse}
%&\frac{T \vdash e_{1} \rightarrow T \vdash e_{1}'}
%{T \vdash if \; e_{1} \; then \; e_{2} \; else \; e_{3} \rightarrow T \vdash if \; e_{1}' \; then \; e_{2} \; else \; e_{3}}\\ \\
%\tag{E-PairLeft}
%&\frac{T \vdash e_{1} \rightarrow T \vdash e_{1}'}
%{T \vdash (e_{1},e_{2}) \rightarrow T \vdash (e_{1}',e_{2})} \\ \\
%\tag{E-PairRight}
%&\frac{T \vdash e_{2} \rightarrow T \vdash e_{2}'}
%{T \vdash (e_{1},e_{2}) \rightarrow T \vdash (e_{1},e_{2}')} \\ \\
\tag{E-Let}
&\frac{T \vdash e_{1}\rightarrow T \vdash e_{1}'}
{T \vdash let \; p \; = \; e_{1} \; in \; e_{2} \rightarrow T \vdash let \; p \; = \; e_{1}' \; in \; e_{2}}
\\ \\
\tag{E-LetV}
&T \vdash let \; id \; = \; v \; in \; e \rightarrow T \vdash [id \mapsto v]e \\ \\
%\tag{E-LetRec}
%& T \vdash letrec\;p=\;e_{1} \; in \; e_{2} \rightarrow T \vdash let \; p \; = %fix(\lambda p.e_{1}') \; in \; e_{2} \\ \\ 
%\tag{E-Fix}
%&\frac{T \vdash e\rightarrow T \vdash e'}
%{T \vdash fix(e) \rightarrow T \vdash fix(e')}\\ \\
%\tag{E-FixRec}
%&T \vdash fix(\lambda(p.e)) \rightarrow T \vdash [p \mapsto (fix %(\lambda(p.e))]e \\
\\
\tag{E-PatternMatch}
&T \vdash let \; (p_{1},p_{2}) \; = \; (e_{1},e_{2}) \; in \; e_{3} \rightarrow
let \; p_{1} \; = \; e_{1} \; in \;
(let \; p_{2}  \; = \; e_{2} \; in \; e_{3}) \\ \\
\tag{E-App1}
&\frac{T \vdash e_{1} \rightarrow T \vdash e_{1}'}
{T \vdash e_{1} e_{2} \rightarrow T \vdash e_{1}' e_{2}}\\ \\
\tag{E-App2}
&\frac{T \vdash e_{2} \rightarrow T \vdash e_{2}'}
{T \vdash v\;e_{2} \rightarrow T \vdash v\;e_{2}'}\\ \\
\tag{E-Lambda}
&T \vdash (\lambda x . e) \; v \rightarrow T \vdash [x \mapsto v]e \\ \\
\tag{E-MatchLambda}
&T \vdash (\lambda (p_{1},p_{2}) . e_{3}) \; (e_{1},e_{2}) \rightarrow T \vdash (\lambda p_{1}.(\lambda p_{2}.e_{3})\;e_{2})\; e_{1} \\
%\displaybreak
\\
\tag{E-ModVar}
&\frac{\longspace (x=e':\tau) \in T[M_{i}].\overline{d} \longspace e=[this.y\mapsto M.y]e'\;\forall (this.y \in e')}
{T \vdash M.x \rightarrow T \vdash e}\\
\\
%\tag{E-FunVar}
%&\frac{\longspace (x=e':\tau) \in T[F_{i}].\overline{d} \longspace %e=[M_{1..n} \mapsto M_{args}][this.y\mapsto F_{i}%(\overline{M_{args}}).y]e'\;\forall (this.y \in e')}
%{T \vdash F_{1}(\overline{M_{args}}).x \rightarrow T \vdash e}
\end{align*}
\caption{\MiniML\ evaluation rules.\label{fig:MiniMLOperationalSemantics}}
\end{figure}
